MirrorCharge!/src/OrderedCanceller.v
@@ -1,0 +1,476 @@
+(** This is a simple cancellation procedure based on
+ ** an ordering of the elements on the right hand side.
+ **)
+Require Import ExtLib.Tactics.
+Require Import MirrorCore.TypesI.
+Require Import MirrorCore.SymI.
+Require Import MirrorCore.Subst.
+Require Import MirrorCore.Ext.Expr.
+Require Import MirrorCore.Ext.AppFull.
+Require Import MirrorCore.Ext.ExprSem.
+Require Import MirrorCore.EnvI.
+Require Import ILogic BILogic Pure.
+Require Import BILNormalize.
+Require Import Iterated.
+Require Import SynSepLog.
+
+Set Implicit Arguments.
+Set Strict Implicit.
+
+Section ordered_cancel.
+  Variable ts : types.
+  Variable func : Type.
+  Variable RSym_func : RSym (typD ts) func.
+
+  Inductive Conjuncts : Type :=
+  | Pure (_ : expr func) (c : Conjuncts)
+  | Impure (f : expr func) (xs : list (expr func)) (c : Conjuncts)
+  | Emp
+  | Tru.
+
+  Variable subst : Type.
+  Variable Subst_subst : Subst subst (expr func).
+  Hypothesis SubstOk_subst : SubstOk _ Subst_subst.
+
+  Fixpoint findWithRest {T U} (f : T -> option U) (ls acc : list T) {struct ls}
+  : option (T * U * list T) :=
+    match ls with
+      | nil => None
+      | l :: ls =>
+        match f l with
+          | None => findWithRest f ls (l :: acc)
+          | Some u => Some (l, u, rev_append acc ls)
+        end
+    end.
+
+  Theorem findWithRest_spec
+  : forall T U f ls acc a s b,
+      @findWithRest T U f ls acc = Some (a,s,b) ->
+      f a = Some s /\
+      exists before after,
+        b = before ++ after /\ rev_append acc ls = before ++ a :: after.
+  Proof.
+    clear. induction ls; simpl; intros; try congruence.
+    consider (f a); intros.
+    { inv_all; subst. split; auto.
+      exists (rev acc). exists ls.
+      repeat rewrite rev_append_rev. auto. }
+    { eapply IHls in H0. intuition. }
+  Qed.
+
+  Variable doUnifySepLog : subst -> expr func -> expr func -> option subst.
+
+  Fixpoint cancel (rhs : Conjuncts) (lhs : conjunctives func)
+           (rem : conjunctives func) (s : subst) {struct rhs}
+  : conjunctives func * conjunctives func * subst :=
+    match rhs with
+      | Emp => (lhs, rem, s)
+      | Tru => (lhs, {| spatial := rem.(spatial)
+                      ; pure := rem.(pure)
+                      ; star_true := true
+                      |}, s)
+      | Pure p cs =>
+        cancel cs lhs {| spatial := rem.(spatial)
+                       ; star_true := rem.(star_true)
+                       ; pure := p :: rem.(pure)
+                       |} s
+      | Impure f xs cs =>
+        let Z := apps f xs in
+        let test x := doUnifySepLog s Z (apps (fst x) (snd x)) in
+        match findWithRest test lhs.(spatial) nil with
+          | None =>
+            cancel cs lhs {| spatial := (f,xs) :: rem.(spatial)
+                           ; star_true := rem.(star_true)
+                           ; pure := rem.(pure)
+                           |} s
+          | Some (_, s', rst) =>
+            cancel cs {| spatial := rst
+                       ; star_true := lhs.(star_true)
+                       ; pure := lhs.(pure)
+                       |}
+                      rem s'
+        end
+    end.
+
+  Variable tySL : typ.
+  Variable ILogicOps_SL : ILogicOps (typD ts nil tySL).
+  Variable BILOperators_SL : BILOperators (typD ts nil tySL).
+  Hypothesis ILogic_SL : @ILogic _ ILogicOps_SL.
+  Hypothesis BILogic_SL : @BILogic _ ILogicOps_SL BILOperators_SL.
+
+  Variable us vs : EnvI.env (typD ts).
+
+  (** TODO: this can be generalized to handle entailment with a remainder **)
+  Hypothesis doUnifySepLogOk : forall s e e' s',
+    doUnifySepLog s e e' = Some s' ->
+    WellTyped_expr (typeof_env us) (typeof_env vs) e tySL ->
+    WellTyped_expr (typeof_env us) (typeof_env vs) e' tySL ->
+    WellTyped_subst (typeof_env us) (typeof_env vs) s ->
+    substD us vs s' ->
+    exprD us vs e tySL = exprD us vs e' tySL /\
+    substD us vs s.
+
+
+  Variable SSL : SynSepLog func.
+  Variable SSLO : SynSepLogOk _ _ _ _ SSL.
+
+  Fixpoint ConjunctsD (ls : Conjuncts) : option (typD ts nil tySL) :=
+    match ls with
+      | Emp => Some empSP
+      | Tru => Some ltrue
+      | Pure p ls =>
+        match exprD us vs p tySL , ConjunctsD ls with
+          | Some a , Some b => Some (sepSP (land a empSP) b)
+          | _ , _ => None
+        end
+      | Impure f xs ls =>
+        match exprD us vs (apps f xs) tySL , ConjunctsD ls with
+          | Some a , Some b => Some (sepSP a b)
+          | _ , _ => None
+        end
+    end.
+
+  Variable PureOp_SL : @Pure.PureOp (typD ts nil tySL).
+  Variable Pure_SL : Pure.Pure PureOp_SL.
+  Hypothesis Pure_ltrue : Pure.pure ltrue.
+
+  Fixpoint well_formed_Conjuncts (ls : Conjuncts) : Prop :=
+    match ls with
+      | Emp => True
+      | Tru => True
+      | Pure p ls =>
+        match exprD us vs p tySL with
+          | None => False
+          | Some p => Pure.pure p
+        end /\ well_formed_Conjuncts ls
+      | Impure _ _ ls => well_formed_Conjuncts ls
+    end.
+
+  Fixpoint Conjuncts_to_expr (ls : Conjuncts) : expr func :=
+    match ls with
+      | Emp => SSL.(e_emp)
+      | Tru => SSL.(e_true)
+      | Pure p ls =>
+        SSL.(e_star) (SSL.(e_and) p SSL.(e_emp)) (Conjuncts_to_expr ls)
+      | Impure f xs ls =>
+        SSL.(e_star) (apps f xs) (Conjuncts_to_expr ls)
+    end.
+
+
+  Definition sentails : env (typD ts) -> env (typD ts) -> expr func -> expr func -> Prop :=
+    @Sem_equiv ts func _ tySL lentails.
+
+  Lemma exprD'_iterated_base_cons_Some
+  : forall us tvs a b x,
+      exprD' us tvs (iterated_base SSL.(e_emp) SSL.(e_star) (a :: b)) tySL = Some x ->
+      exists aV bV,
+        exprD' us tvs a tySL = Some aV /\
+        exprD' us tvs (iterated_base SSL.(e_emp) SSL.(e_star) b) tySL = Some bV /\
+        (forall vs, ((x vs) -|- sepSP (aV vs) (bV vs))).
+  Proof.
+    clear Pure_SL PureOp_SL Pure_ltrue.
+    unfold iterated_base. simpl.
+    intros.
+    destruct (iterated (e_star SSL) b).
+    { go_crazy SSL SSLO; eauto. }
+    { exists x.
+      destruct (SSLO.(e_empOk) us0 tvs) as [ ? [ ? ? ] ].
+      eexists x0. split; auto. split; auto. intros.
+      rewrite H1. rewrite empSPR; eauto. }
+  Qed.
+
+  Lemma exprD'_iterated_base_cons_None
+  : forall us tvs a b,
+      exprD' us tvs (iterated_base SSL.(e_emp) SSL.(e_star) (a :: b)) tySL = None <->
+      exprD' us tvs a tySL = None \/
+      exprD' us tvs (iterated_base SSL.(e_emp) SSL.(e_star) b) tySL = None.
+  Proof.
+    clear Pure_SL PureOp_SL Pure_ltrue.
+    unfold iterated_base. simpl.
+    intros.
+    destruct (iterated (e_star SSL) b); auto.
+    { split; intros; repeat (go_crazy SSL SSLO); auto.
+      consider (exprD' us0 tvs (e_star SSL a e) tySL); intros; auto.
+      exfalso. go_crazy SSL SSLO. destruct H; congruence. }
+    { split; intros; repeat (go_crazy SSL SSLO); auto.
+      destruct H; auto.
+      exfalso.
+      destruct (SSLO.(e_empOk) us0 tvs). intuition. congruence. }
+  Qed.
+
+
+  Lemma exprD'_iterated_base_app_Some
+  : forall us tvs a b x,
+      exprD' us tvs (iterated_base SSL.(e_emp) SSL.(e_star) (a ++ b)) tySL = Some x ->
+      exists aV bV,
+        exprD' us tvs (iterated_base SSL.(e_emp) SSL.(e_star) a) tySL = Some aV /\
+        exprD' us tvs (iterated_base SSL.(e_emp) SSL.(e_star) b) tySL = Some bV /\
+        (forall vs, ((x vs) -|- sepSP (aV vs) (bV vs))).
+  Proof.
+    clear Pure_SL PureOp_SL doUnifySepLogOk Pure_ltrue.
+    induction a; simpl; intros.
+    { destruct (SSLO.(e_empOk) us0 tvs) as [ ? [ ? ? ] ].
+      exists x0. exists x.
+      split; eauto. split; eauto.
+      intros. rewrite H1. rewrite empSPL. reflexivity. }
+    { eapply exprD'_iterated_base_cons_Some in H.
+      destruct H as [ ? [ ? [ ? [ ? ? ] ] ] ].
+      specialize (IHa _ _ H0).
+      destruct IHa as [ ? [ ? [ ? [ ? ? ] ] ] ].
+      consider (exprD' us0 tvs (iterated_base (e_emp SSL) (e_star SSL) (a :: a0)) tySL); intros.
+      { do 2 eexists. split; eauto. split; eauto.
+        apply exprD'_iterated_base_cons_Some in H5.
+        destruct H5 as [ ? [ ? [ ? [ ? ? ] ] ] ].
+        intros. Cases.rewrite_all_goal.
+        rewrite H in *. rewrite H6 in *.
+        inv_all; subst.
+        rewrite sepSPA. reflexivity. }
+      { exfalso.
+        eapply exprD'_iterated_base_cons_None in H5.
+        destruct H5; congruence. } }
+  Qed.
+
+  Lemma exprD'_iterated_base_app_None
+  : forall us tvs a b,
+      exprD' us tvs (iterated_base SSL.(e_emp) SSL.(e_star) (a ++ b)) tySL = None <->
+      exprD' us tvs (iterated_base SSL.(e_emp) SSL.(e_star) a) tySL = None \/
+      exprD' us tvs (iterated_base SSL.(e_emp) SSL.(e_star) b) tySL = None.
+  Proof.
+    clear Pure_SL PureOp_SL doUnifySepLogOk Pure_ltrue.
+    induction a; simpl; intros.
+    { intuition.
+      unfold iterated_base in H0. simpl in *.
+      destruct (SSLO.(e_empOk) us0 tvs) as [ ? [ ? ? ] ].
+      congruence. }
+    { repeat rewrite exprD'_iterated_base_cons_None.
+      rewrite IHa. split; tauto. }
+  Qed.
+
+  Lemma cancelOk_lem
+  : forall rhs lhs rem s lhs' rhs' s',
+      cancel rhs lhs rem s = (lhs',rhs',s') ->
+      well_formed _ _ _ lhs us vs ->
+      well_formed_Conjuncts rhs ->
+      well_formed _ _ _ rem us vs ->
+      sentails us vs (conjunctives_to_expr_star SSL lhs')
+                     (conjunctives_to_expr_star SSL rhs') ->
+      match exprD us vs (conjunctives_to_expr_star SSL lhs) tySL
+          , exprD us vs (SSL.(e_star) (conjunctives_to_expr_star SSL rem)
+                                      (Conjuncts_to_expr rhs)) tySL
+      with
+        | Some l , Some r => l |-- r
+        | _ , _ => True
+      end.
+  Proof.
+    unfold sentails.
+    induction rhs; intros.
+    { simpl in H.
+      specialize (IHrhs _ _ _ _ _ _ H H0).
+      simpl in H1. forward. destruct H4.
+      (** TODO: this is about provability and it isn't implemented yet **)
+      admit. }
+    { simpl in H.
+      match goal with
+        | _ : match ?X with _ => _ end = _ |- _ =>
+          consider X
+      end; intros.
+      { destruct p. destruct p.
+        forward.
+        red in H3. unfold Sem_equiv, exprD in *.
+        destruct (split_env vs).
+        forward. inv_all; subst. simpl in *.
+        repeat (go_crazy SSL SSLO).
+        assert (well_formed RSym_func tySL PureOp_SL
+            {| spatial := l; star_true := star_true lhs; pure := pure lhs |}
+            us vs).
+        { destruct lhs. simpl in *. auto. }
+        assert (well_formed_Conjuncts rhs).
+        { simpl in *; auto. }
+        assert (well_formed RSym_func tySL PureOp_SL rem us vs) by auto.
+        specialize (IHrhs _ _ _ _ _ _ H4 H11 H12 H13 H3); clear H11 H12 H13 H3 H4.
+        repeat go_crazy SSL SSLO.
+        inv_all; subst.
+        eapply findWithRest_spec in H.
+        destruct H. destruct H3 as [ ? [ ? [ ? ? ] ] ].
+        simpl in *. subst.
+        unfold conjunctives_to_expr_star in *.
+        repeat (go_crazy SSL SSLO).
+        rewrite H11 in *.
+        rewrite map_app in H16.
+        apply exprD'_iterated_base_app_Some in H16.
+        simpl in *.
+        repeat match goal with
+                 | H : _ /\ _ |- _ => destruct H
+                 | H : exists x, _ |- _ => destruct H
+               end.
+        eapply exprD'_iterated_base_cons_Some in H20.
+        repeat match goal with
+                 | H : _ /\ _ |- _ => destruct H
+                 | H : exists x, _ |- _ => destruct H
+               end.
+        consider (exprD' us x
+                (e_star SSL
+                   (iterated_base (e_emp SSL) (e_star SSL)
+                      (map (e_and SSL (e_emp SSL)) (pure lhs)))
+                   (e_star SSL
+                      (iterated_base (e_emp SSL) (e_star SSL)
+                         (map
+                            (fun x : expr func * list (expr func) =>
+                             apps (fst x) (snd x))
+                            (x0 ++ x3)))
+                      (if star_true lhs then e_true SSL else e_emp SSL)))
+                tySL).
+        { intros. clear H11.
+          repeat go_crazy SSL SSLO.
+          inv_all; subst.
+          rewrite map_app in H24.
+          eapply exprD'_iterated_base_app_Some in H24.
+          destruct H24 as [ ? [ ? [ ? [ ? ? ] ] ] ].
+          repeat go_crazy SSL SSLO.
+          inv_all; subst.
+          Cases.rewrite_all_goal.
+          assert (x17 h ** (x19 h ** x11 h ** x14 h ** x22 h) |--
+                  x2 h ** (x7 h ** x9 h ** x10 h ** x6 h)).
+          { apply scME.
+            { admit. }
+            { etransitivity. etransitivity.
+              2: eapply IHrhs.
+              clear IHrhs. Cases.rewrite_all_goal.
+              repeat rewrite sepSPA. reflexivity.
+              clear IHrhs. Cases.rewrite_all_goal.
+              repeat rewrite sepSPA. reflexivity. } }
+          { etransitivity. etransitivity. 2: eapply H11.
+            repeat rewrite <- sepSPA.
+            { apply scME; try reflexivity.
+              apply scME; try reflexivity.
+              rewrite sepSPC. rewrite sepSPA. reflexivity. }
+            { repeat rewrite <- sepSPA.
+              apply scME; try reflexivity.
+              rewrite sepSPC with (Q := x2 h).
+              repeat rewrite sepSPA.
+              reflexivity. } } }
+        { intros.
+          clear H25.
+          repeat go_crazy SSL SSLO.
+          rewrite map_app in H24.
+          apply exprD'_iterated_base_app_None in H24.
+          destruct H24; congruence. } }
+      { (** findWithRest returns None **)
+        unfold Sem_equiv in *.
+        forward.
+        assert (well_formed RSym_func tySL PureOp_SL lhs us vs) by auto.
+        assert (well_formed_Conjuncts rhs) by auto.
+        assert (well_formed RSym_func tySL PureOp_SL
+                            {|
+                              spatial := spatial rem;
+                              star_true := star_true rem;
+                              pure := pure rem |} us vs) by auto.
+        specialize (IHrhs _ _ _ _ _ _ H4 H7 H8 H9 H3); clear H4 H3 H7 H8 H9.
+        rewrite H5 in *. simpl in *. clear H.
+        consider (exprD us vs
+              (e_star SSL
+                 (conjunctives_to_expr_star SSL
+                    {|
+                    spatial := (f,xs) :: spatial rem;
+                    star_true := star_true rem;
+                    pure := pure rem |}) (Conjuncts_to_expr rhs)) tySL); intros.
+        { rewrite IHrhs; clear IHrhs H5 t.
+          unfold conjunctives_to_expr_star in *; simpl in *.
+          unfold exprD in *.
+          destruct (split_env vs).
+          forward.
+          inv_all; subst.
+          destruct rem; simpl in *.
+          repeat go_crazy SSL SSLO.
+          inv_all; subst.
+          apply exprD'_iterated_base_cons_Some in H14.
+          destruct H14 as [ ? [ ? [ ? [ ? ? ] ] ] ].
+          rewrite H6 in *. rewrite H3 in *.
+          inv_all; subst.
+          Cases.rewrite_all_goal.
+          repeat rewrite <- sepSPA.
+          apply scME; try reflexivity.
+          repeat rewrite sepSPA.
+          apply scME; try reflexivity.
+          rewrite sepSPC. rewrite sepSPA.
+          reflexivity. }
+        { clear H3.
+          unfold conjunctives_to_expr_star in *. simpl in *.
+          unfold exprD in *.
+          destruct (split_env vs). forward.
+          inv_all; subst.
+          repeat (go_crazy SSL SSLO; try congruence).
+          eapply exprD'_iterated_base_cons_None in H.
+          destruct H; congruence. } } }
+    { simpl in *.
+      inv_all; subst.
+      forward.
+      red in H3.
+      unfold exprD in *.
+      destruct (split_env vs).
+      forward. inv_all; subst.
+      destruct (SSLO.(e_empOk) us x) as [ ? [ ? ? ] ].
+      repeat go_crazy SSL SSLO.
+      inv_all; subst.
+      Cases.rewrite_all_goal.
+      rewrite empSPR by eauto with typeclass_instances.
+      reflexivity. }
+    { simpl in *.
+      inv_all; subst.
+      red in H3. unfold exprD in *. forward.
+      inv_all; subst.
+      destruct (SSLO.(e_trueOk) us x) as [ ? [ ? ? ] ].
+      repeat go_crazy SSL SSLO.
+      inv_all; subst.
+      rewrite H4; clear H4 H3.
+      destruct rem.
+      unfold conjunctives_to_expr_star in *. simpl in *.
+      repeat go_crazy SSL SSLO.
+      inv_all; subst.
+      Cases.rewrite_all_goal.
+      repeat rewrite sepSPA.
+      apply scME; try reflexivity.
+      apply scME; try reflexivity.
+      destruct star_true.
+      { rewrite H8 in *. inv_all; subst.
+        Cases.rewrite_all.
+        eapply ltrue_sep; eauto with typeclass_instances. }
+      { destruct (SSLO.(e_empOk) us x).
+        rewrite H8 in *.
+        destruct H3.
+        inv_all; subst.
+        rewrite H4. rewrite empSPL. apply ltrueR. } }
+  Qed.
+
+  Variable order : conjunctives func -> Conjuncts.
+(*
+  Hypothesis orderOk : forall c us vs,
+    well_formed _ c us vs ->
+    sentails (Conjuncts_to_expr (order c)) (conjunctives_to_expr c).
+*)
+
+  Definition ordered_cancel (lhs rhs : conjunctives func) (s : subst)
+  : conjunctives func * conjunctives func * subst :=
+    let ordered := order rhs in
+    let empty := {| spatial := nil ; pure := nil ; star_true := false |} in
+    cancel ordered lhs empty s.
+
+End ordered_cancel.
+
+(** The simplest ordering heuristic just uses the order that they occur in the
+ ** map without looking at unification variables.
+ **)
+Section simple_ordering.
+  Variable typ : Type.
+  Variable typD : list Type -> typ -> Type.
+  Variable RType_typ : RType typD.
+  Variable func : Type.
+  Variable RSym_func : RSym typD func.
+
+  Definition order_conjunctives (c : conjunctives func) : Conjuncts func :=
+    List.fold_right (fun x acc => Impure (fst x) (snd x) acc)
+                    (List.fold_right (fun x acc => Pure x acc)
+                                     (if c.(star_true) then Tru _ else Emp _)
+                                     c.(pure))
+                    c.(spatial).
+End simple_ordering.
